updates

Veritas.Verifier.Global.fst
@@ -104,18 +104,66 @@ let lemma_g_hadd_correct (gl: verifiable_log):
   Lemma (hadd gl = ms_hashfn (g_add_seq gl)) =
   lemma_g_hadd_correct_aux gl
 
+let rec add_set_map_aux (gl: verifiable_log) (ii: sseq_index gl {is_blum_add (indexss gl ii)}):
+  Tot (j: seq_index (g_add_seq gl){index (g_add_seq gl) j = blum_add_elem (indexss gl ii)}) 
+  (decreases (length gl)) =
+  let (tid,i) = ii in
+  let p = length gl in
+  let gl' = prefix gl (p - 1) in
+  let s' = g_add_seq gl' in
+  let tl = thread_log gl (p - 1) in
+
+  if tid = p - 1 then
+    length s' + (VT.add_seq_map tl i)  
+  else
+    add_set_map_aux gl' ii
+  
 let add_set_map (gl: verifiable_log) (ii: sseq_index gl {is_blum_add (indexss gl ii)}):
-  (j: seq_index (g_add_seq gl){index (g_add_seq gl) j = blum_add_elem (indexss gl ii)}) = admit()
+  (j: seq_index (g_add_seq gl){index (g_add_seq gl) j = blum_add_elem (indexss gl ii)}) = 
+  add_set_map_aux gl ii
+
+(* inverse mapping from add_seq to the blum add entries in the verifier logs *)
+let rec add_set_map_inv_aux (gl: verifiable_log) (j: seq_index (g_add_seq gl)):
+  Tot (ii: sseq_index gl {is_blum_add (indexss gl ii) /\ add_set_map gl ii = j})
+  (decreases (length gl)) = 
+  let p = length gl in
+  let gl' = prefix gl (p - 1) in
+  let s' = g_add_seq gl' in
+  let tl = thread_log gl (p - 1) in  
+  let s = g_add_seq gl in
+
+  if j < length s' then 
+    add_set_map_inv_aux gl' j  
+  else 
+    let j' = j - length s' in
+    let i = VT.add_seq_inv_map tl j' in
+    (p-1, i)  
 
 (* inverse mapping from add_seq to the blum add entries in the verifier logs *)
 let add_set_map_inv (gl: verifiable_log) (j: seq_index (g_add_seq gl)):
   (ii: sseq_index gl {is_blum_add (indexss gl ii) /\ 
-                      add_set_map gl ii = j}) = admit()
+                      add_set_map gl ii = j}) = 
+  add_set_map_inv_aux gl j                      
+
+let rec lemma_add_set_map_inv_aux (gl: verifiable_log)(ii: sseq_index gl {is_blum_add (indexss gl ii)}):
+  Lemma (requires True)
+        (ensures (add_set_map_inv gl (add_set_map gl ii) = ii))
+        (decreases (length gl)) =
+  let (tid,i) = ii in
+  let p = length gl in
+  let gl' = prefix gl (p - 1) in
+  let s' = g_add_seq gl' in
+  let tl = thread_log gl (p - 1) in
+
+  if tid = p - 1 then ()
+  else
+    lemma_add_set_map_inv_aux gl' ii
 
 let lemma_add_set_map_inv (gl: verifiable_log)(ii: sseq_index gl {is_blum_add (indexss gl ii)}):
   Lemma (requires True)
         (ensures (add_set_map_inv gl (add_set_map gl ii) = ii))
-        [SMTPat (add_set_map gl ii)] = admit()
+        [SMTPat (add_set_map gl ii)] = 
+  lemma_add_set_map_inv_aux gl ii
 
 let rec g_evict_seq_aux (gl: verifiable_log):
   Tot (seq (ms_hashfn_dom))
